books/projects/apply/all-warrants-valid.lisp
@@ -1,0 +1,171 @@
+; Copyright (C) 2016, ForrestHunt, Inc.
+; Written by Matt Kaufmann and J Moore
+; License: A 3-clause BSD license.  See the LICENSE file distributed with ACL2.
+
+; Portcullis:
+; (include-book "evaluation-lemmas")
+
+; Verification that All the Warrants in User-Book.lisp Are Valid in
+;               the Evaluation Theory Produced by the
+;  Defattaches of their Doppelgangers to BADGE-USERFN and APPLY$-USERFN
+
+(in-package "ACL2")
+
+(defthm apply$-warrant-AP-valid
+  (apply$-warrant-AP)
+  :hints
+  (("Goal" :in-theory (enable apply$-warrant-ap))))
+
+(defthm apply$-warrant-REV-valid
+  (apply$-warrant-REV)
+  :hints
+  (("Goal" :in-theory (enable apply$-warrant-rev))))
+
+(defthm apply$-warrant-PALINDROMIFY-LIST-valid
+  (apply$-warrant-PALINDROMIFY-LIST)
+  :hints
+  (("Goal" :in-theory (enable apply$-warrant-palindromify-list))))
+
+(defthm apply$-warrant-LIST-OF-TRUE-LISTSP-valid
+  (apply$-warrant-LIST-OF-TRUE-LISTSP)
+  :hints
+  (("Goal" :in-theory (enable apply$-warrant-list-of-true-listsp))))
+
+(defthm apply$-warrant-LIST-OF-LIST-OF-TRUE-LISTSP-valid
+  (apply$-warrant-LIST-OF-LIST-OF-TRUE-LISTSP)
+  :hints
+  (("Goal" :in-theory (enable apply$-warrant-list-of-list-of-true-listsp))))
+
+(defthm apply$-warrant-EXPT-5-valid
+  (apply$-warrant-EXPT-5)
+  :hints
+  (("Goal" :in-theory (enable apply$-warrant-EXPT-5))))
+
+(defthm apply$-warrant-OK-FNP-valid
+  (apply$-warrant-OK-FNP)
+  :hints
+  (("Goal" :in-theory (enable apply$-warrant-ok-fnp))))
+
+(defthm apply$-warrant-COLLECT-valid
+  (apply$-warrant-COLLECT)
+  :hints
+  (("Goal" :in-theory (e/d (apply$-warrant-collect)
+                           (collect-is-a-foldr)))))
+
+(defthm apply$-warrant-SUMLIST-valid
+  (apply$-warrant-SUMLIST)
+  :hints
+  (("Goal" :in-theory (e/d (apply$-warrant-sumlist)
+                           (sumlist-is-a-foldr)))))
+
+(defthm apply$-warrant-SUMLIST-WITH-PARAMS-valid
+  (apply$-warrant-SUMLIST-WITH-PARAMS)
+  :hints
+  (("Goal" :in-theory (enable apply$-warrant-sumlist-with-params))))
+
+(defthm apply$-warrant-FILTER-valid
+  (apply$-warrant-FILTER)
+  :hints
+  (("Goal" :in-theory (enable apply$-warrant-filter))))
+
+(defthm apply$-warrant-ALL-valid
+  (apply$-warrant-ALL)
+  :hints
+  (("Goal" :in-theory (e/d (apply$-warrant-all)
+                           (all-is-a-foldr)))))
+
+(defthm apply$-warrant-COLLECT-ON-valid
+  (apply$-warrant-COLLECT-ON)
+  :hints
+  (("Goal" :in-theory (enable apply$-warrant-collect-on))))
+
+(defthm apply$-warrant-COLLECT-TIPS-valid
+  (apply$-warrant-COLLECT-TIPS)
+  :hints
+  (("Goal" :in-theory (enable apply$-warrant-collect-tips))))
+
+(defthm apply$-warrant-APPLY$2-valid
+  (apply$-warrant-APPLY$2)
+  :hints
+  (("Goal" :in-theory (enable apply$-warrant-apply$2))))
+
+(defthm apply$-warrant-APPLY$2x-valid
+  (apply$-warrant-APPLY$2x)
+  :hints
+  (("Goal" :in-theory (enable apply$-warrant-apply$2x))))
+
+(defthm apply$-warrant-APPLY$2xx-valid
+  (apply$-warrant-APPLY$2x)
+  :hints
+  (("Goal" :in-theory (enable apply$-warrant-apply$2xx))))
+
+(defthm apply$-warrant-RUSSELL-valid
+  (apply$-warrant-RUSSELL)
+  :hints
+  (("Goal" :in-theory (enable apply$-warrant-russell))))
+
+(defthm apply$-warrant-FOLDR-valid
+  (apply$-warrant-FOLDR)
+  :hints
+  (("Goal" :in-theory (enable apply$-warrant-foldr))))
+
+(defthm apply$-warrant-FOLDL-valid
+  (apply$-warrant-FOLDL)
+  :hints
+  (("Goal" :in-theory (enable apply$-warrant-foldl))))
+
+(defthm apply$-warrant-COLLECT-FROM-TO-valid
+  (apply$-warrant-COLLECT-FROM-TO)
+  :hints
+  (("Goal" :in-theory (enable apply$-warrant-collect-from-to))))
+
+(defthm apply$-warrant-COLLECT*-valid
+  (apply$-warrant-COLLECT*)
+  :hints
+  (("Goal" :in-theory (enable apply$-warrant-COLLECT*))))
+
+(defthm apply$-warrant-COLLECT2-valid
+  (apply$-warrant-COLLECT2)
+  :hints
+  (("Goal" :in-theory (enable apply$-warrant-COLLECT2))))
+
+(defthm apply$-warrant-RECUR-BY-COLLECT-valid
+  (apply$-warrant-RECUR-BY-COLLECT)
+  :hints
+  (("Goal" :in-theory (enable apply$-warrant-RECUR-BY-COLLECT))))
+
+(defthm apply$-warrant-PROW-valid
+  (apply$-warrant-PROW)
+  :hints
+  (("Goal" :in-theory (enable apply$-warrant-PROW))))
+
+(defthm apply$-warrant-PROW*-valid
+  (apply$-warrant-PROW*)
+  :hints
+  (("Goal" :in-theory (enable apply$-warrant-PROW*))))
+
+(defthm apply$-warrant-FN-5-valid
+  (apply$-warrant-FN-5)
+  :hints
+  (("Goal" :in-theory (enable apply$-warrant-FN-5))))
+
+(defthm apply$-warrant-MAP-FN-5-valid
+  (apply$-warrant-MAP-FN-5)
+  :hints
+  (("Goal" :in-theory (enable apply$-warrant-MAP-FN-5))))
+
+(defthm apply$-warrant-SUMLIST-EXPR-valid
+  (apply$-warrant-SUMLIST-EXPR)
+  :hints
+  (("Goal" :in-theory (enable apply$-warrant-SUMLIST-EXPR))))
+
+(defthm apply$-warrant-COLLECT-REV-valid
+  (apply$-warrant-COLLECT-REV)
+  :hints
+  (("Goal" :in-theory (enable apply$-warrant-COLLECT-REV))))
+
+(defthm apply$-warrant-SUM-OF-PRODUCTS-valid
+  (apply$-warrant-SUM-OF-PRODUCTS)
+  :hints
+  (("Goal" :in-theory (enable apply$-warrant-SUM-OF-PRODUCTS))))
+
