books/projects/apply/copy-file.lisp
@@ -1,0 +1,40 @@
+; Copyright (C) 2016, ForrestHunt, Inc.
+; Written by Matt Kaufmann and J Moore
+; License: A 3-clause BSD license.  See the LICENSE file distributed with ACL2.
+
+; Portcullis: 
+; Empty
+
+; Copy-file
+
+; (copy-file name1 name2 state) copies the file named name1 to a file named name2.
+; It opens and closes the channels it creates.
+
+(in-package "ACL2")
+
+(set-state-ok t)
+
+(defun copy-file1 (channel1 channel2 state)
+  (declare (xargs :mode :program))
+  (mv-let (byte state)
+    (read-byte$ channel1 state)
+    (cond
+     ((null byte) state)
+     (t (let ((state (write-byte$ byte channel2 state)))
+          (copy-file1 channel1 channel2 state))))))
+
+(defun copy-file (file1 file2 state)
+  (declare (xargs :mode :program))
+  (mv-let (channel1 state)
+    (open-input-channel file1 :byte state)
+    (mv-let (channel2 state)
+      (open-output-channel file2 :byte state)
+      (let* ((state (copy-file1 channel1 channel2 state))
+             (state (close-output-channel channel2 state))
+             (state (close-input-channel channel1 state)))
+        state))))
+
+
+
+
+
