books/projects/apply/defattach-demo.lisp
@@ -1,0 +1,103 @@
+; Copyright (C) 2016, ForrestHunt, Inc.
+; Written by Matt Kaufmann and J Moore
+; License: A 3-clause BSD license.  See the LICENSE file distributed with ACL2.
+
+; Portcullis:
+; (include-book "user-book")
+; (include-book "doppelgangers")
+; (defattach badge-userfn badge-userfn!)
+; (defattach apply$-userfn apply$-userfn!)
+
+; A Demonstration of the Evaluation Theory Produced by the Defattaches Above
+
+(in-package "ACL2")
+
+; This book demonstrates that we can successfully attach the doppelgangers to
+; the four apply$ stubs.  Of course, that is not a hard goal to achieve since
+; the constraints on the stubs are so weak.  But the defattaches below justify
+; our later consideration of an evaluation theory containing the four
+; corresponding attachment equations.  After the four attachments we show that
+; a couple of examples evaluate as we expect.
+
+(defmacro expected-to (expectation theory form val)
+
+; This macro is just a convenient way of evaluating the translation of form in
+; either the current theory or the evaluation theory and testing whether the
+; result is val.  The result can thus fail in two ways: (a) form's translation
+; and/or evaluation causes an error or (b) form's translation and evaluation
+; return a value different from val.  Expectation is :fail or :succeed and
+; indicates whether we expect the evaluation to fail or succeed.  Theory is
+; either :current or :evaluation.
+
+  `(,(if (eq expectation :fail) 'must-fail 'must-succeed)
+    (er-let*
+      ((pair (simple-translate-and-eval
+              ',form
+              nil nil "Help!" 'ctx (w state) state
+              ,(if (eq theory :current) nil t) ; = aok
+              )))
+      (cond
+       ((equal (cdr pair) ,val) (value t))
+       (t (mv t nil state))))))
+
+; Because apply$ is not evaluable in the current theory, the following will fail.
+
+(expected-to :fail :current
+             (collect '((1 2 3) (4 5 6))
+                      '(lambda (x)
+                         (COLLECT (REV x)
+                                  '(lambda (y) (cons 'a y)))))
+             '(((A . 3) (A . 2) (A . 1))
+               ((A . 6) (A . 5) (A . 4))))
+
+; However, the equivalence can be proved in the current theory if we have the
+; right warrants:
+
+(defthm demo-of-collect-eval-by-rewriting
+  (implies (and (apply$-warrant-COLLECT)
+                (apply$-warrant-REV))
+           (equal (collect '((1 2 3) (4 5 6))
+                           '(LAMBDA (X)
+                              (COLLECT (REV X)
+                                       '(LAMBDA (Y) (CONS 'A Y)))))
+                  '(((A . 3) (A . 2) (A . 1))
+                    ((A . 6) (A . 5) (A . 4)))))
+  :hints (("Goal" :expand ((:free (x) (HIDE x))))))
+
+; The warrants for COLLECT and REV are necessary because those symbols appear
+; inside the quoted LAMBDA and are thus ultimately apply$'d.  (The collect
+; outside the LAMBDA is just part of an ACL2 term, not something concerning
+; apply$ or ev$.
+
+; While we cannot evaluate the collect expression above in the current theory
+; we can do so in the evaluation theory because we've done the defattaches in
+; the portcullis.
+
+(expected-to :succeed :evaluation
+             (collect '((1 2 3) (4 5 6))
+                      '(LAMBDA (X)
+                         (COLLECT (REV X)
+                                  '(LAMBDA (Y) (CONS 'A Y)))))
+             '(((A . 3) (A . 2) (A . 1))
+               ((A . 6) (A . 5) (A . 4))))
+
+; Here is another sample evaluation in the evaluation theory, this
+; time using collect and FOLDR.
+
+(expected-to :succeed :evaluation
+             (collect '((1) (1 2) (1 2 3) (1 2 3 4 5))
+                      '(LAMBDA (LST) (FOLDR LST 'BINARY-* '1)))
+             '(1 2 6 120))
+
+; Expt-2-and-expt-3 has no warrant.  So (badge 'EXPT-2-EXPT-3) is not what you
+; might expect (even though a badge for it is recorded in the badge-table).  In
+; fact, calling badge on 'EXPT-2-AND-EXPT-3 causes an evaluation error.
+
+(expected-to :fail :evaluation
+             (badge 'EXPT-2-AND-EXPT-3)
+             '(APPLY$-BADGE NIL 1 . T))
+
+(expected-to :succeed :evaluation
+             (badge 'expt-5)
+             '(APPLY$-BADGE T 1 . T))
+
