books/projects/apply/evaluation-lemmas.lisp
@@ -1,0 +1,232 @@
+; Copyright (C) 2016, ForrestHunt, Inc.
+; Written by Matt Kaufmann and J Moore
+; License: A 3-clause BSD license.  See the LICENSE file distributed with ACL2.
+
+; Portcullis:
+; (include-book "evaluation-user-book")
+
+; Lemmas Needed to Prove that the Warrants of User-Book are Valid
+
+; The book basically just proves, for every function fn that has a doppelganger
+; fn!, that fn!=fn, in the evaluation theory of
+; (defattach badge-userfn badge-userfn!)
+; (defattach apply$-userfn apply$-userfn!)
+; after defining all the doppelgangers of user-book.lisp.
+
+; That evaluation theory is realized as a current theory by
+; (defun badge-userfn (fn) (badge-userfn! fn))
+; (defun apply$-userfn (fn args) (apply$-userfn! fn args))
+; and then re-certifying apply.lisp and user-book.lisp.  That's
+; how evaluation-user-book.lisp, in the portcullis above, was built.
+
+(in-package "ACL2")
+
+(include-book "tools/flag" :dir :system)
+
+(defthm badge-is-badge!
+  (equal (badge fn) (badge! fn))
+  :hints (("Goal" :in-theory (enable badge badge!))))
+
+(make-flag boom tamep)
+(defthm-boom
+  (defthm tamep-is-tamep!
+    (equal (tamep x) (tamep! x))
+    :flag tamep)
+  (defthm tamep-functionp-is-tamep-functionp!
+    (equal (tamep-functionp fn) (tamep-functionp! fn))
+    :flag tamep-functionp)
+  (defthm suitably-tamep-listp-is-suitably-tamep-listp!
+    (equal (suitably-tamep-listp n flags args) (suitably-tamep-listp! n flags args))
+    :flag suitably-tamep-listp))
+
+(make-flag bang apply$!
+           :hints (("Goal" :in-theory (enable badge apply$))))
+
+; The following represents a lemma we may need to prove that
+; recur-by-collect is equal to its doppleganger.
+
+(defthm len-collect
+  (equal (len (collect lst fn))
+         (len lst))
+  :hints
+  (("Goal" :in-theory (disable collect-is-a-foldr))))
+
+(defthm len-prow
+  (implies (not (endp (cdr lst)))
+           (< (len (prow lst fn))(len lst)))
+  :rule-classes :linear)
+
+(defthm-bang
+  (defthm apply$!-is-apply$
+    (equal (apply$! fn args) (apply$ fn args))
+    :flag apply$!)
+
+; BTW: The proofs of these theorems illustrate why we need the tamep in ev$ (a
+; question we were once uncertain about).  When evaluating a call of a
+; user-defined mapper, ev$! just cadrs the functional arg but ev$ evaluates it.
+; But that means that apply$!  is apply$ on lambda applications only if the
+; body is tame!
+
+  (defthm ev$!-is-ev$
+    (equal (ev$! x a) (ev$ x a))
+    :flag ev$!)
+  (defthm ev$!-list-is-ev$-list
+    (equal (ev$!-list x a) (ev$-list x a))
+    :flag ev$!-list)
+  (defthm collect!-is-collect
+    (equal (collect! lst fn)
+           (collect lst fn))
+    :flag collect!)
+  (defthm sumlist!-is-sumlist
+    (equal (sumlist! lst fn)
+           (sumlist lst fn))
+    :flag sumlist!)
+  (defthm sumlist-with-params!-is-sumlist
+    (equal (sumlist-with-params! lst fn params)
+           (sumlist-with-params lst fn params))
+    :flag sumlist-with-params!)
+  (defthm filter!-is-filter
+    (equal (filter! lst fn)
+           (filter lst fn))
+    :flag filter!)
+  (defthm all!-is-all
+    (equal (all! lst fn)
+           (all lst fn))
+    :flag all!)
+  (defthm collect-on!-is-collect-on
+    (equal (collect-on! lst fn)
+           (collect-on lst fn))
+    :flag collect-on!)
+  (defthm collect-tips!-is-collect-tips
+    (equal (collect-tips! x fn)
+           (collect-tips x fn))
+    :flag collect-tips!)
+  (defthm apply$2!-is-apply$2
+    (equal (apply$2! fn x y)
+           (apply$2 fn x y))
+    :flag apply$2!)
+  (defthm apply$2x!-is-apply$2x
+    (equal (apply$2x! fn x y)
+           (apply$2x fn x y))
+    :flag apply$2x!)
+  (defthm apply$2xx!-is-apply$2xx
+    (equal (apply$2xx! fn x y)
+           (apply$2xx fn x y))
+    :flag apply$2xx!)
+  (defthm russell!-is-russell
+    (equal (russell! fn x)
+           (russell fn x))
+    :flag russell!)
+  (defthm foldr!-is-foldr
+    (equal (foldr! lst fn init)
+           (foldr lst fn init))
+    :flag foldr!)
+  (defthm foldl!-is-foldl
+    (equal (foldl! lst fn ans)
+           (foldl lst fn ans))
+    :flag foldl!)
+  (defthm collect-from-to!-is-collect-from-to
+    (equal (collect-from-to! i max fn)
+           (collect-from-to i max fn))
+    :flag collect-from-to!)
+  (defthm collect*!-is-collect
+    (equal (collect*! lst fn)
+           (collect* lst fn))
+    :flag collect*!)
+  (defthm collect2!-is-collect
+    (equal (collect2! lst fn1 fn2)
+           (collect2 lst fn1 fn2))
+    :flag collect2!)
+  (defthm recur-by-collect!-is-recur-by-collect
+    (equal (recur-by-collect! lst fn)
+           (recur-by-collect lst fn))
+    :flag recur-by-collect!)
+  (defthm prow!-is-prow
+    (equal (prow! lst fn)
+           (prow lst fn))
+    :flag prow!)
+  (defthm prow*!-is-prow*
+    (equal (prow*! lst fn)
+           (prow* lst fn))
+    :flag prow*!)
+  (defthm fn-2-and-fn-3!-is-fn-2-and-fn-3
+    (equal (fn-2-and-fn-3! fn x)
+           (fn-2-and-fn-3 fn x))
+    :flag fn-2-and-fn-3!)
+  (defthm fn-5!-is-fn-5
+    (equal (fn-5! fn x)
+           (fn-5 fn x))
+    :flag fn-5!)
+  (defthm map-fn-5!-is-fn-5
+    (equal (map-fn-5! lst fn)
+           (map-fn-5 lst fn))
+    :flag map-fn-5!)
+  (defthm sumlist-expr!-is-sumlist-expr
+    (equal (sumlist-expr! lst expr alist)
+           (sumlist-expr lst expr alist))
+    :flag sumlist-expr!)
+  :hints
+  (("Goal"
+    :in-theory (enable badge apply$ ev$ apply$-lambda)
+    :expand (
+             (ev$! x a)
+             (ev$ x a)
+             (:free (n ilk ilks x) (suitably-tamep-listp! n (cons ilk ilks) x))
+             (COLLECT-FROM-TO! I MAX FN)
+             (COLLECT-FROM-TO I MAX FN)
+             ))
+   ))
+
+(defthm apply$-lambda!-is-apply$-lambda
+  (equal (apply$-lambda! fn args) (apply$-lambda fn args)))
+
+; =================================================================
+; 13. prove that the dopplegangers of the ordinary functions and tame
+;     instances are equal to their correspondents.
+
+(defthm ap!-is-ap
+  (equal (ap! x y)
+         (ap x y)))
+
+(defthm rev!-is-rev
+  (equal (rev! x)
+         (rev x)))
+
+(defthm palindromify-list!-is-palindromify-list
+  (equal (palindromify-list! lst)
+         (palindromify-list lst)))
+
+(defthm list-of-true-listsp!-is-list-of-true-listsp
+  (equal (list-of-true-listsp! lst)
+         (list-of-true-listsp lst)))
+
+(defthm list-of-list-of-true-listsp!-is-list-of-list-of-true-listsp
+  (equal (list-of-list-of-true-listsp! lst)
+         (list-of-list-of-true-listsp lst)))
+
+(defthm expt-2-and-expt-3!-is-expt-2-and-expt-3
+  (equal (expt-2-and-expt-3! x)
+         (expt-2-and-expt-3 x)))
+
+(defthm expt-5!-is-expt-5
+  (equal (expt-5! x)
+         (expt-5 x)))
+
+(defthm ok-fnp!-is-ok-fnp
+  (equal (ok-fnp! lst)
+         (ok-fnp lst)))
+
+(defthm collect-rev!-is-collect-rev
+  (equal (collect-rev! x)
+         (collect-rev x))
+  :hints (("Goal" :in-theory (e/d (APPLY$) (APPLY$-REV)))))
+
+(defthm sum-of-products!-is-sum-of-products
+  (equal (sum-of-products! x)
+         (sum-of-products x))
+  :hints (("Goal" :in-theory (e/d (APPLY$) (APPLY$-REV)))))
+
+; =================================================================
+; The End
+
+
