books/projects/apply/foldr-exercises.lisp
@@ -1,0 +1,245 @@
+; Copyright (C) 2016, ForrestHunt, Inc.
+; Written by Matt Kaufmann and J Moore
+; License: A 3-clause BSD license.  See the LICENSE file distributed with ACL2.
+
+; Portcullis:
+; (include-book "apply")
+
+; FOLDR Exercises
+
+; Summary
+
+; In this book we define the classic function FOLDR and prove that various
+; familiar functions and ideas can be expressed with it.  In particular, we
+; show how FOLDR can ``be'' APPEND, REV, COLLECT, ALLWAYS, SUMLIST, FILTER, and
+; (sort of) MAXLIST.
+
+; Some implications of this work are:
+
+; (1) We might consider providing FOLDR as a primitive and then not allowing
+; the user to define any mappers (i.e., prevent the user from using APPLY$ etc
+; in defuns) and just rely on FOLDR to provide a lot of power and convenience.
+; This would simplify the soundness story considerably because then we would
+; not have to contemplate finding a measure (in the model construction as
+; illustrated by modeled-portculis.lisp) for arbitrary mapping functions.  We'd
+; support just APPLY$, EV$, EV$-LIST, and FOLDR.  Instead, we find a measure to
+; explain APPLY$, EV$, EV$-LIST, and FOLDR and that measure and clique is fixed
+; for all instances of the story.  (Personally, Moore isn't persuaded that we
+; want to prohibit the definition of other mappers.)
+
+; (2) However, maybe there is a way to use FOLDR to create a simpler soundness
+; story while still allowing the user to define COLLECT, etc.  For example, in
+; the soundness story we could keep the concrete clique fixed as in (2) and
+; model COLLECT and the all the other user-defined mappers as calls of FOLDR,
+; which removes them from the clique and allows us to skip the creation of the
+; messy measure.  Of course, to rely on this version of the story we'd want to
+; check that every user-defined mapper was really some instance of FOLDR, a not
+; unreasonable restriction.
+
+; (3) At one point below (see maxlist-non-nil and maxlist-is-sort-of-a-foldr)
+; we have to express the idea that fn returns an integer on every element of a
+; given list and we do this with ALLWAYS and COLLECT.  It is very natural in
+; the sense that it was easy to write, the normal machinery handled its
+; participation in the proofs, and it avoids the definition of yet another
+; special-purpose recursive function.  Thus, these exercises can be thought of
+; as a little supporting evidence for the utility of apply and mapping
+; functions.
+
+; (ld "~/work/apply/book1/consistency/foldr-exercises.lisp")
+; (certify-book "foldr-exercises")
+
+(in-package "ACL2")
+
+; (include-book "apply")
+
+(defun$ foldr (lst fn init)
+  (if (endp lst)
+      init
+      (apply$ fn
+              (list (car lst)
+                    (foldr (cdr lst) fn init)))))
+(defun$ ap (x y)
+  (if (consp x)
+      (cons (car x) (ap (cdr x) y))
+      y))
+
+(defun$ rev (x)
+  (if (consp x)
+      (ap (rev (cdr x)) (cons (car x) nil))
+      nil))
+
+(defthm foldr-is-ap
+  (equal (foldr x 'cons y) (ap x y)))
+
+(defthm foldr-is-rev
+  (implies (apply$-warrant-foldr)
+           (equal (foldr x
+                         '(lambda (x y)
+                                  (foldr y 'cons (cons x 'nil)))
+                         nil)
+                  (rev x))))
+
+; Now I define various mappers and show that foldr can be made to
+; do all those jobs.
+
+(defun$ collect (lst fn)
+  (cond ((endp lst) nil)
+        (t (cons (apply$ fn (list (car lst)))
+                 (collect (cdr lst) fn)))))
+
+(defun$ allways (lst fn)
+  (cond ((endp lst) t)
+        (t (and (apply$ fn (list (car lst)))
+                (allways (cdr lst) fn)))))
+
+(defun$ sumlist (lst fn)
+  (cond ((endp lst) 0)
+        (t (+ (apply$ fn (list (car lst)))
+              (sumlist (cdr lst) fn)))))
+
+(defun$ max$ (x y)
+
+; I have to define max$ rather than use the built-in MAX because the current
+; APPLY$ does not consider MAX built-in!  Remember, the current APPLY$ only
+; recognizes the primitives in *apply$-primitives*.
+
+  (if (< x y) y x))
+
+(defun$ maxlist (lst fn)
+  (cond ((endp lst) nil)
+        ((endp (cdr lst)) (apply$ fn (list (car lst))))
+        (t (max$ (apply$ fn (list (car lst)))
+                 (maxlist (cdr lst) fn)))))
+
+(defun$ filter (lst fn)
+  (cond ((endp lst) nil)
+        ((apply$ fn (list (car lst)))
+         (cons (car lst) (filter (cdr lst) fn)))
+        (t (filter (cdr lst) fn))))
+
+; The theorem below, which is not being stored as a rule, illustrates the most
+; general fact we can think of relating COLLECT and FOLDR:
+
+(defthm general-collect-is-a-foldr
+  (implies (and (not (equal fn 'QUOTE))
+                (not (equal fn 'IF))
+                (symbolp x)
+                (symbolp y)
+                (not (eq x y))
+                (tamep `(,fn ,x)))
+           (equal (collect lst fn)
+                  (foldr lst
+                         `(lambda (,x ,y)
+                            (cons (,fn ,x) ,y))
+                         nil)))
+  :rule-classes nil)
+
+; But this rule is not useful as a rewrite rule because x and y are free
+; variables.  Furthermore, if the goal is to rewrite COLLECTs into FOLDRs, it's
+; not necessary to be so general.  We can just choose the x and y we want to
+; use.  We use a convenient abbreviation for the hypotheses we'll see over and
+; over here.
+
+(defun$ ok-fnp (fn)
+  (and (not (equal fn 'QUOTE))
+       (not (equal fn 'IF))
+       (tamep `(,fn X))))
+
+(defthm collect-is-a-foldr
+  (implies (force (ok-fnp fn))
+           (equal (collect lst fn)
+                  (foldr lst
+                         `(LAMBDA (X Y)
+                                  (CONS (,fn X) Y))
+                         nil))))
+
+(defthm allways-is-a-foldr
+  (implies (force (ok-fnp fn))
+           (equal (allways lst fn)
+                  (foldr lst
+                         `(LAMBDA (X Y)
+                                  (IF (,fn X) Y 'NIL))
+                         t))))
+
+(defthm sumlist-is-a-foldr
+  (implies (force (ok-fnp fn))
+           (equal (sumlist lst fn)
+                  (foldr lst
+                         `(LAMBDA (X Y)
+                                  (BINARY-+ (,fn X) Y))
+                         0))))
+
+; Clearly we could on and on with these sorts of mappers!
+
+; Before dealing with maxlist we deal with filter...
+
+(defthm filter-is-a-foldr
+  (implies (force (ok-fnp fn))
+           (equal (filter lst fn)
+                  (foldr lst `(lambda (x y)
+                                (if (,fn x)
+                                    (cons x y)
+                                    y))
+                         nil))))
+
+; Maxlist cannot be expressed as a foldr without some additional hypotheses or
+; special cases.  The problem is that maxlist never calls itself recursively on
+; the empty list while foldr does.  That means maxlist never compares its
+; ``initial value'' (i.e., its value on the empty list) to any of the values
+; returned by fn.  But foldr does compare those two.  One can try to avoid that
+; by special-casing the singleton list sort of like maxlist does, but in fact
+; that idea doesn't work.  (Note the NOT in the conclusion; the theorem below
+; provides a counterexample to the claimed equivalence.)
+
+(defthm maxlist-is-not-this-foldr!
+  (let ((lst '(4 1))
+        (fn '(lambda (x) (binary-* '-5 x))))
+    (implies (and (force (ok-fnp fn))
+                  (apply$-warrant-MAX$)
+                  )
+             (NOT (equal (maxlist lst fn)
+                         (if (endp lst)
+                             nil
+                             (if (endp (cdr lst))
+                                 (apply$ fn (list (car lst)))
+                                 (foldr lst
+                                        `(LAMBDA (X Y)
+                                                 (MAX$ (,fn X) Y))
+                                        nil)))))))
+  :hints (("Goal" :expand ((:free (x) (HIDE x)))))
+  :rule-classes nil)
+
+; The maxlist above returns -5 but the foldr returns nil (which is bigger than
+; all the negatives).
+
+; So if foldr always compares its value on the empty list to the values of fn
+; on elements of its input list, we must have a way to tell whether the value
+; being compared is the special one returned for the empty list.  But without
+; some kind of restriction on what fn returns, we cannot designate a
+; ``special'' value.
+
+; If we posit that fn always returns a number (at least, over the elements in
+; lst), then we can tell the difference between the initial value and any call
+; of fn, and then we get a reasonable relationship.
+
+(defthm maxlist-non-nil
+  (implies (and (force (ok-fnp fn))
+                (allways (collect lst fn) 'acl2-numberp))
+           (iff (maxlist lst fn)
+                (consp lst))))
+
+(defthm maxlist-is-sort-of-a-foldr
+  (implies (and (force (ok-fnp fn))
+                (apply$-warrant-MAX$)
+                (allways (collect lst fn) 'acl2-numberp))
+           (equal (maxlist lst fn)
+                  (foldr lst `(lambda (x y)
+                                (if (equal y 'nil) 
+                                    (,fn x)
+                                    (max$ (,fn x) y)))
+                         nil))))
+
+; This concludes our foldr exercises.
+
+
+
